ulib/FStar.HyperStack.ST.fst
@@ -748,7 +748,8 @@ let lemma_witnessed_constant (p:Type0)
 let lemma_witnessed_nested (p:mem_predicate)
   :Lemma (witnessed (fun (m:mem) -> witnessed p) <==> witnessed p)
   = W.lemma_witnessed_nested mem_rel p;
-    assert (FStar.FunctionalExtensionality.feq (fun (m:mem) -> witnessed p) (fun (m:mem) -> W.witnessed mem_rel p))
+    assert (FStar.FunctionalExtensionality.feq (fun (m:mem) -> witnessed p) (fun (m:mem) -> W.witnessed mem_rel p));
+    assume ((fun (m:mem) -> witnessed p) == (fun (m:mem) -> W.witnessed mem_rel p))
 
 let lemma_witnessed_and (p q:mem_predicate)
   :Lemma (witnessed (fun s -> p s /\ q s) <==> (witnessed p /\ witnessed q))
